theories/Trans.v
@@ -1098,3 +1098,5 @@ Proof.
   - apply trans_vis_inv in TR.
     destruct TR as (? & ? & abs); inv abs.
 Qed.
+
+
